state/SharedRefs.fsti
@@ -3,30 +3,44 @@ module SharedRefs
 open FStar.Tactics
 
 open FStar.Preorder
-open FStar.Monotonic.Heap
+include FStar.Monotonic.Heap
 open FStar.Ghost
-open MST.Tot
+include MST.Tot
 
-type map_sharedT = mref (pos -> GTot bool) (fun (m0 m1:pos -> GTot bool) -> forall p. m0 p ==> m1 p) (** pre-order necessary to show that the predicate `is_shared` is stable **)
+type ref_pred =
+  #a:Type0 -> #rel:preorder a -> mref a rel -> Type0
+
+type ref_heap_stable_pred =
+  pred:(#a:Type -> #rel:_ -> mref a rel -> heap -> Type0){forall (a:Type) (x:ref a) h0 h1. pred x h0 /\ h0 `heap_rel` h1 ==> pred x h1}
+
+type map_sharedT = 
+  mref (pos -> GTot bool) (fun (m0 m1:pos -> GTot bool) -> forall p. m0 p ==> m1 p) (** pre-order necessary to show that the predicate `is_shared` is stable **)
 
 noeq
 type sigT = {
   map_shared : erased map_sharedT;
-  is_shared : #a:Type0 -> #p:preorder a -> mref a p -> h:heap -> Type0;
-  is_shared_stable : #a:Type0 -> r:ref a -> Lemma (stable (is_shared r)) [SMTPat (is_shared r)];
+  is_shared : pred:ref_heap_stable_pred;
+ // is_shared_implies_contained : #a:_ -> #rel:_ -> r:mref a rel -> h:heap -> Lemma (is_shared r h ==> h `contains` r);
+  fresh_ref_not_shared : #a:_ -> #rel:_ -> (r:mref a rel) -> h:heap -> Lemma (
+    (forall p. p >= next_addr h ==> ~((sel h map_shared) p)) /\ (addr_of r >= next_addr h) ==> ~(is_shared r h));
+  unmodified_map_implies_same_shared_status : s:Set.set nat -> h0:heap -> h1:heap -> 
+    Lemma (h0 `contains` map_shared /\ h0 `heap_rel` h1 /\ ~(addr_of map_shared `Set.mem` s) /\ modifies s h0 h1 ==> 
+      (forall #a #rel (r:mref a rel). is_shared r h0 <==> is_shared r h1));
+  same_addr_same_sharing_status : #aa:_ -> #rela:_ -> #b:_ -> #relb:_ -> ra:mref aa rela -> rb:mref b relb -> h:heap ->
+    Lemma (addr_of ra == addr_of rb ==> (is_shared ra h <==> is_shared rb h));
   share : #a:Type0 -> #p:preorder a -> sr:(mref a p) ->
     ST unit 
       (requires (fun h0 -> 
         h0 `contains` sr /\
         h0 `contains` map_shared /\
-        (addr_of sr =!= addr_of map_shared) /\ (** prevent sharing the map *)
-        ~(is_shared (map_shared) h0) /\
+        ~(compare_addrs sr map_shared) /\ (** prevent sharing the map *)
+        ~(is_shared map_shared h0) /\
         (forall p. p >= next_addr h0 ==> ~(sel h0 map_shared p)))) (** necessary to prove that freshly allocated references are not shared **)
       (ensures (fun h0 _ h1 ->
         modifies !{map_shared} h0 h1 /\
         ~(is_shared (map_shared) h1) /\
         (forall b (r:ref b). is_shared r h0 ==> is_shared r h1) /\
-        (forall b (r:ref b). ~(is_shared r h0) /\ addr_of r =!= addr_of sr ==> ~(is_shared r h1)) /\
+        (forall b (r:ref b). ~(is_shared r h0) /\ ~(compare_addrs r sr) ==> ~(is_shared r h1)) /\
         (forall p. p >= next_addr h1 ==> ~(sel h1 map_shared p)) /\
         is_shared sr h1))
 }
@@ -40,19 +54,275 @@ unfold let unmodified_common (h0:heap) (h1:heap) : Type0 =
                                r `unused_in` h1 ==> r `unused_in` h0) /\
   (forall (n: nat) . {:pattern (n `addr_unused_in` h0) }
     n `addr_unused_in` h1 ==> n `addr_unused_in` h0)
+
 let modifies_only_shared (h0:heap) (h1:heap) : Type0 =
   (forall (a:Type) (rel:preorder a) (r:mref a rel).{:pattern (sel h1 r)} 
     (h0 `contains` r /\ ~(shareS.is_shared r h0)) ==> sel h0 r == sel h1 r) /\
   unmodified_common h0 h1
 
+type inv_typ =
+  | IUnit
+  | INat
+  | ISum : inv_typ -> inv_typ -> inv_typ
+  | IPair : inv_typ -> inv_typ -> inv_typ
+  | IRef : inv_typ -> inv_typ
+  | ILList : inv_typ -> inv_typ
+
+let rec to_Type (t:inv_typ) : Type u#0 = 
+  match t with
+  | IUnit -> unit
+  | INat -> int
+  | ISum t1 t2 -> either (to_Type t1) (to_Type t2)
+  | IPair t1 t2 -> (to_Type t1) * (to_Type t2)
+  | IRef t -> ref (to_Type t)
+  | ILList t -> linkedList (to_Type t)
+
+let rec forallRefs (pred:ref_pred) (#t:inv_typ) (x:to_Type t) : Type0 =
+  let rcall #t x = forallRefs pred #t x in
+  match t with
+  | IUnit -> True
+  | INat -> True
+  | ISum t1 t2 -> begin
+    let x : either (to_Type t1) (to_Type t2) = x in
+    match x  with
+    | Inl x' -> rcall x' 
+    | Inr x' -> rcall x' 
+  end
+  | IPair t1 t2 ->
+    let x : (to_Type t1) * (to_Type t2) = x in
+    rcall (fst x) /\ rcall (snd x)
+  | IRef t' -> 
+    let x : ref (to_Type t') = x in
+    pred #(to_Type t') #(fun _ _ -> True) x
+  | ILList t' -> begin
+    let x : linkedList (to_Type t') = x in
+    match x with
+    | LLNil -> True
+    | LLCons v xsref -> 
+      rcall v /\ pred xsref
+   end 
+
+let forallRefsHeap (pred:ref_heap_stable_pred) (h:heap) (#t:inv_typ) (x:to_Type t) : Type0 =
+  forallRefs (fun r -> pred r h) x
+
+let lemma_forallRefs (t:inv_typ) (x:to_Type (IRef t)) (pred:ref_pred) :
+  Lemma (forallRefs pred x == pred x) [SMTPat (forallRefs pred x)] by (compute ()) = ()
+  
+let lemma_forallRefsHeap (t:inv_typ) (x:to_Type (IRef t)) (pred:ref_heap_stable_pred) (h:heap) :
+  Lemma (forallRefsHeap pred h x == pred x h) [SMTPat (forallRefsHeap pred h x)] by (compute ()) = ()
+
+let rec forallRefsHeap_monotonic (pred:ref_heap_stable_pred) (h0 h1:heap) (#t:inv_typ) (x:to_Type t) :
+  Lemma (h0 `heap_rel` h1 /\ forallRefsHeap pred h0 x ==> forallRefsHeap pred h1 x) =
+  match t with
+  | IUnit -> ()
+  | INat -> ()
+  | ISum t1 t2 -> begin
+    let x : either (to_Type t1) (to_Type t2) = x in
+    match x  with
+    | Inl x' -> forallRefsHeap_monotonic pred h0 h1 x' 
+    | Inr x' -> forallRefsHeap_monotonic pred h0 h1 x' 
+  end
+  | IPair t1 t2 ->
+    let x : (to_Type t1) * (to_Type t2) = x in
+    forallRefsHeap_monotonic pred h0 h1 (fst x);
+    forallRefsHeap_monotonic pred h0 h1 (snd x) 
+  | IRef t' -> ()
+  | ILList t' -> begin
+    let x : linkedList (to_Type t') = x in
+    match x with
+    | LLNil -> ()
+    | LLCons v xsref -> 
+      forallRefsHeap_monotonic pred h0 h1 v 
+   end 
+
+let ctrans_ref_pred (h:heap) (pred:ref_heap_stable_pred) =
+  (** forall references, if r satisfies pred in h, then the references r points to also satisfy pred **)
+  (forall (t:inv_typ) (r:ref (to_Type t)).
+    pred r h ==> forallRefsHeap pred h (sel h r))
+  // CA: previous version tried to implement this with typeclasses, but it was not working because one had to prove 
+  // that two instances of the same type are equal.
+  // invariant:
+  //   forall (a:Type) (c:witnessable a) (r:ref a). 
+  //     (witnessable_ref _ #c).satisfy r h pred ==> c.satisfy (sel h r) h pred
+  // lemma needed:
+  //   forall (a:Type) (c:witnessable a) (c':witnessable a) (r:ref a).
+  //     c.satisfy r h pred ==> c'.satisfy r h pred
+
+let trans_shared_contains (h:heap) = 
+  ctrans_ref_pred h contains_pred /\ ctrans_ref_pred h shareS.is_shared
+
 effect IST (a:Type) (pre:st_pre) (post: (h:heap -> Tot (st_post' a (pre h)))) =
   ST a 
-    (requires (fun h0      -> 
+    (requires (fun h0 -> 
+      trans_shared_contains h0 /\
       h0 `contains` shareS.map_shared /\ 
       ~(shareS.is_shared (shareS.map_shared) h0) /\ (* the map stays unshared *)
       (forall p. p >= next_addr h0 ==> ~(sel h0 shareS.map_shared p)) /\
       pre h0))
     (ensures  (fun h0 r h1 -> 
+      trans_shared_contains h1 /\
       ~(shareS.is_shared (shareS.map_shared) h1) /\
       (forall p. p >= next_addr h1 ==> ~(sel h1 shareS.map_shared p)) /\
       post h0 r h1))
+
+let eliminate_ctrans_ref_pred (h:heap) a (r:ref (to_Type a)) (pred:ref_heap_stable_pred) :
+  Lemma
+    (requires (ctrans_ref_pred h pred))
+    (ensures (pred r h ==> forallRefsHeap pred h (sel h r)
+    )) = ()
+
+let eliminate_ctrans_ref_shared h a (r:ref (to_Type a)) :
+  Lemma
+    (requires (ctrans_ref_pred h shareS.is_shared))
+    (ensures (shareS.is_shared r h ==> forallRefsHeap shareS.is_shared h (sel h r))) = ()
+
+let eliminate_ctrans_ref_contains h a (r:ref (to_Type a)) :
+  Lemma
+    (requires (ctrans_ref_pred h contains_pred))
+    (ensures (contains_pred r h ==> forallRefsHeap contains_pred h (sel h r))) = ()
+
+let rec inversion (a:inv_typ) (xa:inv_typ) :
+  Lemma
+    (requires (to_Type a == to_Type xa))
+    (ensures (a == xa)) =
+  match a with
+  | IUnit -> ()
+  | INat -> ()
+  | _ -> admit ()
+
+let read (#t:inv_typ) (r:ref (to_Type t)) 
+  : IST (to_Type t) 
+        (requires (fun h0 -> h0 `contains` r))
+        (ensures (fun h0 v h1 -> h0 == h1 /\ v == sel h1 r)) =
+  MST.Tot.read r
+  
+let lemma_ist_alloc_preserves_contains t (x:ref (to_Type t)) (v:to_Type t) (h0 h1:heap) : Lemma
+  (requires (
+    h0 `heap_rel` h1 /\
+    h1 == upd h0 x v /\ 
+    fresh x h0 h1 /\ 
+    modifies Set.empty h0 h1 /\
+    sel h1 x == v /\ 
+    ~(shareS.is_shared x h1) /\
+    is_mm x == false /\
+    forallRefsHeap contains_pred h0 v /\
+    ctrans_ref_pred h0 contains_pred))
+  (ensures (
+    ctrans_ref_pred h1 contains_pred)) = 
+  introduce forall a (r:ref (to_Type a)).
+      contains_pred r h1 ==> forallRefsHeap contains_pred h1 (sel h1 r)
+  with begin
+    introduce contains_pred r h1 ==> forallRefsHeap contains_pred h1 (sel h1 r)
+    with _. begin
+      introduce addr_of r =!= addr_of x ==> forallRefsHeap contains_pred h1 (sel h1 r) with _. begin
+        eliminate_ctrans_ref_pred h0 a r contains_pred;
+        assert (h0 `contains` r);
+        forallRefsHeap_monotonic contains_pred h0 h1 (sel h0 r)
+      end;
+      introduce addr_of r == addr_of x ==> forallRefsHeap contains_pred h1 (sel h1 r) with _. begin
+        assert (sel h1 x == v);
+        inversion a t;
+        forallRefsHeap_monotonic contains_pred h0 h1 v
+      end
+    end
+  end
+
+let lemma_ist_alloc_preserves_shared t (x:ref (to_Type t)) (v:to_Type t) (h0 h1:heap) : Lemma
+  (requires (
+    h0 `contains` shareS.map_shared /\
+    h0 `heap_rel` h1 /\
+    h1 == upd h0 x v /\ 
+    fresh x h0 h1 /\ 
+    modifies Set.empty h0 h1 /\
+    sel h1 x == v /\ 
+    ~(shareS.is_shared x h1) /\
+    is_mm x == false /\
+    forallRefsHeap contains_pred h0 v /\
+    ctrans_ref_pred h0 shareS.is_shared))
+  (ensures (
+    ctrans_ref_pred h1 shareS.is_shared)) =
+  introduce forall a (r:ref (to_Type a)). shareS.is_shared r h1 ==> forallRefsHeap shareS.is_shared h1 (sel h1 r)
+  with begin
+    introduce shareS.is_shared r h1 ==> forallRefsHeap shareS.is_shared h1 (sel h1 r) with _. begin
+      shareS.unmodified_map_implies_same_shared_status Set.empty h0 h1;
+      assert (shareS.is_shared r h0);
+      eliminate_ctrans_ref_pred h0 a r shareS.is_shared;
+      forallRefsHeap_monotonic shareS.is_shared h0 h1 (sel h0 r);
+      assert (forallRefsHeap shareS.is_shared h1 (sel h0 r));
+      introduce addr_of x =!= addr_of r ==> forallRefsHeap shareS.is_shared h1 (sel h1 r) with _. ();
+      introduce addr_of x == addr_of r ==> forallRefsHeap shareS.is_shared h1 (sel h1 r) with _. begin
+        assert ~(shareS.is_shared x h1);
+        assert (shareS.is_shared r h1);
+        shareS.same_addr_same_sharing_status r x h1;
+        assert False
+      end
+    end
+  end
+
+
+let ist_alloc (#t:inv_typ) (init:to_Type t)
+: IST (ref (to_Type t))
+    (fun h0 -> forallRefsHeap contains_pred h0 init)
+    (fun h0 r h1 -> alloc_post #(to_Type t) init h0 r h1)
+=
+  let h0 = get () in
+  let r = alloc init in
+  let h1 = get () in
+  shareS.fresh_ref_not_shared r h0;
+  shareS.unmodified_map_implies_same_shared_status Set.empty h0 h1;
+  lemma_ist_alloc_preserves_contains t r init h0 h1;
+  lemma_ist_alloc_preserves_shared t r init h0 h1;
+  r
+
+let _ = () 
+
+(**  
+let elab_write (#t:typ0) (r:ref (elab_typ0 t)) (v:elab_typ0 t) 
+: IST unit
+  (requires (fun h0 -> 
+    shallowly_contained_low r #(elab_typ0_tc (TRef t)) h0 /\
+    shallowly_contained_low v #(elab_typ0_tc t) h0))
+  (ensures (fun h0 () h1 ->
+    write_post r v h0 () h1 /\
+    modifies_only_label Low h0 h1 /\
+    shallowly_contained_low r #(elab_typ0_tc (TRef t)) h1))
+= let h0 = get () in
+  write r v;
+  let h1 = get () in
+  lemma_write_preserves_is_low (to_inv_typ t) r v h0 h1;
+  lemma_write_preserves_contains (to_inv_typ t) r v h0 h1;
+  ()
+
+let declassify_low' (#t:typ0) (r:ref (elab_typ0 t)) : ST unit
+  (fun h -> (elab_typ0_tc (TRef t)).satisfy r h contains_pred /\ inv_points_to h contains_pred)
+  (fun h0 () h1 -> 
+    inv_points_to h1 contains_pred /\
+    shallowly_contained_low r #(elab_typ0_tc (TRef t)) h1 /\
+    declassify_post r Low h0 () h1)
+=
+  let h0 = get () in
+  declassify r Low;
+  let h1 = get () in
+  lemma_declassify_preserves_contains (to_inv_typ t) r h0 h1
+
+val elab_alloc (#t:typ0) (init:elab_typ0 t)
+: IST (ref (elab_typ0 t))
+  (requires (fun h0 ->
+    shallowly_contained_low init #(elab_typ0_tc t) h0))
+  (ensures (fun h0 r h1 -> 
+    fresh r h0 h1 /\ 
+    modifies Set.empty h0 h1 /\
+    modifies_classification Set.empty h0 h1 /\
+    sel h1 r == init /\
+    shallowly_contained_low r #(elab_typ0_tc (TRef t)) h1))
+let elab_alloc #t init = 
+  let h0 = get () in
+  let r : ref (elab_typ0 t) = ist_alloc init in
+  let h1 = get () in
+  declassify_low' r;
+  let h2 = get () in
+  (elab_typ0_tc t).satisfy_monotonic init is_low_pred h0 h1;
+  lemma_declassify_preserves_is_low (to_inv_typ t) r h1 h2;
+  assert (inv_points_to h2 is_low_pred);
+  r
+**)
